WIP -- compiles ModSem

theories/Sem.v
@@ -1,10 +1,126 @@
-From Paco Require Import paco.
-Require Import Program.
-Require Import sflib.
+Require Import Coqlib.
+Require Import ITreelib.
 Require Import Universe.
 Require Import STS.
 Require Import Behavior.
 Require Import ModSem.
 Require Import Skeleton.
+Require Import PCM.
+
+Generalizable Variables E R A B C X Y Z.
 
 Set Implicit Arguments.
+
+
+
+Class Dec (A: Type) := dec: forall (a0 a1: A), { a0 = a1 } + { a0 <> a1 }.
+
+Global Program Instance positive_Dec: Dec positive. Next Obligation. decide equality. Defined.
+Global Program Instance string_Dec: Dec string. Next Obligation. apply string_dec. Defined.
+
+Definition update K `{Dec K} V (f: K -> V) (k: K) (v: V): K -> V :=
+  fun _k => if dec k _k then v else f _k.
+
+Notation "f '?'" := (unwrapU f) (at level 60, only parsing).
+Notation "f '﹗'" := (unwrapN f) (at level 60, only parsing).
+
+
+
+Section INTERP.
+
+  Context `{GRA: GRA.t}.
+  Variable ms: ModSem.t.
+
+  Let itr0: callE ~> itree (callE +' mdE +' fnE +' eventE) :=
+    fun _ ce =>
+      trigger FPush;;
+      rv <- (ms.(ModSem.sem) ce);;
+      trigger FPop;;
+      Ret rv
+  .
+  Let itr1: itree (mdE +' fnE +' eventE) val := (mrec itr0) _ (Call "main" nil).
+
+
+
+  Definition md_state: Type := mname -> GRA.
+  Definition handle_mdE `{eventE -< E}: mdE ~> stateT md_state (itree E) :=
+    fun _ e st0 =>
+      match e with
+      | MPut mn gr =>
+        guarantee(RA.updatable (st0 mn) gr);;
+        Ret (update st0 mn gr, tt)
+      | MGet mn => Ret (st0, st0 mn)
+      end.
+  Definition interp_mdE `{eventE -< E}: itree (mdE +' E) ~> stateT md_state (itree E) :=
+    State.interp_state (case_ handle_mdE State.pure_state).
+  Let itr2: itree (fnE +' eventE) val := snd <$> (interp_mdE itr1) (fun _ => URA.unit).
+
+
+
+  Definition fn_state: Type := list GRA.
+  Definition handle_fnE `{eventE -< E}: fnE ~> stateT fn_state (itree E) :=
+    fun _ e st0 =>
+      match e with
+      | FPut gr =>
+        match st0 with
+        | nil => triggerNB
+        | hd :: tl =>
+          guarantee(RA.updatable hd gr);;
+          Ret (gr :: tl, tt)
+        end
+      | FGet =>
+        hd <- (hd_error st0)﹗ ;;
+        Ret (st0, hd)
+      | FPush =>
+        Ret (URA.unit :: st0, tt)
+      | FPop =>
+        Ret (tl st0, tt)
+      end.
+  Definition interp_fnE `{eventE -< E}: itree (fnE +' E) ~> stateT fn_state (itree E) :=
+    State.interp_state (case_ handle_fnE State.pure_state).
+  Let itr3: itree (eventE) val := snd <$> (interp_fnE itr2) nil.
+
+  Let state: Type := itree eventE val.
+
+  Definition state_sort (st0: state): sort :=
+    match (observe st0) with
+    | TauF _ => demonic
+    | RetF rv => final rv
+    | VisF (Choose X) k => demonic
+    | VisF (Take X) k => angelic
+    | VisF (Syscall fn args m0) k => vis
+    end
+  .
+
+  Inductive step: state -> option event -> state -> Prop :=
+  | step_tau
+      itr
+    :
+      step (Tau itr) None itr
+  | step_choose
+      X k (x: X)
+    :
+      step (Vis (subevent _ (Choose X)) k) None (k x)
+  | step_take
+      X k (x: X)
+    :
+      step (Vis (subevent _ (Take X)) k) None (k x)
+  | step_syscall
+      fn args m0 k ev m1 rv
+      (SYSCALL: syscall_sem fn args m0 = (ev, m1, rv))
+    :
+      step (Vis (subevent _ (Syscall fn args m0)) k) (Some ev) (k (m1, rv))
+  .
+
+  Program Definition interp: semantics := {|
+    STS.state := state;
+    STS.step := step;
+    STS.initial_state := itr3;
+    STS.state_sort := state_sort;
+  |}
+  .
+  Next Obligation. inv STEP; inv STEP0; ss. csc. rewrite SYSCALL in *. csc. Qed.
+  Next Obligation. inv STEP; ss. Qed.
+  Next Obligation. inv STEP; ss. Qed.
+
+End INTERP.
